The last admit, no idea what F* is doing

state/Examples.CooperativeMultiThreadingWithIndexT.fst
@@ -59,11 +59,6 @@ let src_run_type (a3p:threep) =
 let run_type_spec (a3p:threep) : spec =
   Spec true true
     (arg_type a3p)
- (**   (witnessable_pair
-      (nat & int)
-      #(witnessable_pair nat #(witnessable_refinement int #witnessable_int _) int #witnessable_int)
-      (l: list (t_task a3p) {List.Tot.Base.length l > 0})
-      #(witnessable_refinement _ #(witnessable_list _ #(witnessable_t_task a3p)) _)) **)
     (importable_pair a3p
 
       (nat & int)
@@ -153,6 +148,26 @@ let run' args = Inl (run args)
 
 let compiled_prog = compile_pprog2 #sit run'
 
+let rec lemma_forall_in_list_true (l:list 'a) :
+  Lemma (forall_in_list l (fun _ -> True)) =
+  match l with
+  | [] -> ()
+  | _::tl -> lemma_forall_in_list_true tl
+
+#set-options "--print_implicits"
+
+  (**
+let rec forall_in_list (l:list 'a) (pred:'a -> Type0) : Type0 =
+  match l with
+  | [] -> True
+  | hd::tl -> pred hd /\ forall_in_list tl pred
+
+let test () : ST unit (fun _ -> True) (fun _ _ _ -> True) =
+  let alloc' () : ST unit (fun _ -> True) (fun _ _ _ -> True) =  let x : ref int = alloc 5 in let _ = read x in () in
+  let alloc'' () : ST unit (fun _ -> True) (fun _ _ _ -> True) = let x : ref int = alloc 5 in () in
+  let l : list (unit -> ST unit (fun _ -> True) (fun _ _ _ -> True)) = [alloc'; alloc''] in
+  assert (forall_in_list l (fun _ -> True))**)
+
 val some_ctx : ctx_tgt2 (comp_int_src_tgt2 sit)
 let some_ctx #a3p read write alloc my_run =
   let res_a : t_task a3p = (fun r () ->
@@ -166,11 +181,33 @@ let some_ctx #a3p read write alloc my_run =
         let () = write r j in
         Return ())) in
 
-  let args : (int * int) * (list (t_task a3p)) = ((5000,0), [res_a; res_b]) in
-  admit (); (**
-      TODO: very hard to debug. My guess was that it fails to show that
-      `satisfy args (prref a3p)`, but from my tests it is not that. **)
-  match my_run args with
+  let my_run123 (x:((int & int) & list (t_task a3p))) : ST (resexn int)
+      (requires (fun h0 -> inv a3p h0 /\ forall_in_list (snd x) (fun _ -> True)))
+      (ensures (post_poly_arrow a3p)) by (
+      norm [delta_only [`%sit;`%comp_int_src_tgt2;`%Mktgt_interface2?.pt;`%Mksrc_interface2?.c_pt;`%exportable_run_type;
+                       `%exportable_arrow_err10;`%mk_exportable;`%Mkexportable_from?.ityp;`%mk_poly_arrow;
+                       `%importable_pair;`%importable_refinement;`%safe_importable_is_importable;`%safe_importable_int;
+                       `%Mkimportable_to?.ityp;`%Mksafe_importable_to?.ityp;
+                       `%poly_iface_is_safely_importable;
+                       `%exportable_int;`%pre_poly_arrow;
+                       `%Mkimportable_to?.c_ityp;`%Mksafe_importable_to?.c_ityp;
+                       `%poly_iface_pair;
+                       `%Mkpoly_iface?.wt;`%witnessable_pair;
+                       `%Mkwitnessable?.satisfy;
+                       `%poly_iface_int;`%witnessable_int;`%poly_iface_list;`%witnessable_list;`%poly_iface_t_task;`%poly_iface_arrow;
+                       `%witnessable_arrow;
+                       ];iota]
+  ) = my_run x in
+
+  let myargs : ((int & int) & list (t_task a3p)) = ((5000,0), [res_a;res_b]) in
+
+  let h = get_heap () in
+  lemma_forall_in_list_true (snd myargs);
+  assume (inv a3p h /\ forall_in_list (snd myargs) (fun _ -> True));
+  (** TODO: the assume is exactly the pre-condition of my_run123 ,
+      and this should not be even assumed because of the lemma. **)
+  admit ();
+  match my_run123 myargs with
   | Inl _ -> 0
   | Inr _ -> -1
 
